proofs/arrays/Array848.ec
@@ -1,0 +1,3 @@
+from Jasmin require import JArray.
+
+clone export PolyArray as Array848  with op size <- 848.
