proofs/arrays/SBArray128_32.ec
@@ -1,0 +1,6 @@
+from Jasmin require import JByte_array.
+
+require import BArray32 BArray128.
+
+clone SubByteArray as SBArray128_32  with theory Asmall <= BArray32,
+                                          theory Abig <= BArray128.
