proofs/arrays/SBArray128_64.ec
@@ -1,0 +1,6 @@
+from Jasmin require import JByte_array.
+
+require import BArray64 BArray128.
+
+clone SubByteArray as SBArray128_64  with theory Asmall <= BArray64,
+                                          theory Abig <= BArray128.
