proofs/arrays/SBArray1952_136.ec
@@ -1,0 +1,6 @@
+from Jasmin require import JByte_array.
+
+require import BArray136 BArray1952.
+
+clone SubByteArray as SBArray1952_136  with theory Asmall <= BArray136,
+                                            theory Abig <= BArray1952.
