proofs/arrays/SBArray1952_48.ec
@@ -1,0 +1,6 @@
+from Jasmin require import JByte_array.
+
+require import BArray48 BArray1952.
+
+clone SubByteArray as SBArray1952_48  with theory Asmall <= BArray48,
+                                           theory Abig <= BArray1952.
