proofs/arrays/SBArray680_136.ec
@@ -1,0 +1,6 @@
+from Jasmin require import JByte_array.
+
+require import BArray136 BArray680.
+
+clone SubByteArray as SBArray680_136  with theory Asmall <= BArray136,
+                                           theory Abig <= BArray680.
