proofs/arrays/SBArray768_136.ec
@@ -1,0 +1,6 @@
+from Jasmin require import JByte_array.
+
+require import BArray136 BArray768.
+
+clone SubByteArray as SBArray768_136  with theory Asmall <= BArray136,
+                                           theory Abig <= BArray768.
