proofs/arrays/SBArray768_16.ec
@@ -1,0 +1,6 @@
+from Jasmin require import JByte_array.
+
+require import BArray16 BArray768.
+
+clone SubByteArray as SBArray768_16  with theory Asmall <= BArray16,
+                                          theory Abig <= BArray768.
