proofs/arrays/SBArray848_168.ec
@@ -1,0 +1,6 @@
+from Jasmin require import JByte_array.
+
+require import BArray168 BArray848.
+
+clone SubByteArray as SBArray848_168  with theory Asmall <= BArray168,
+                                           theory Abig <= BArray848.
