proofs/arrays/WArray848.ec
@@ -1,0 +1,3 @@
+from Jasmin require import JWord_array.
+
+clone export WArray as WArray848  with op size <- 848.
